AP/Util/Array.lean
@@ -2,16 +2,16 @@ import AP.Util.List
 
 namespace Array
 
-variable {α β : Type*} {xs ys : Array α}
+variable {α : Type*} {β : Type*} {xs ys : Array α}
 
-def foldlWith' {β : Sort*} (xs : Array α)
+def foldlWith' (xs : Array α)
 (f : β → (x : α) → x ∈ xs → β) (z : β) (i : ℕ) : β :=
   if h : i < xs.size then xs.foldlWith' f (f z (xs[i]) (by simp)) (i + 1) else z
 
-def foldlWith {β : Sort*} (xs : Array α) (f : β → (x : α) → x ∈ xs → β) (z : β) : β :=
+def foldlWith (xs : Array α) (f : β → (x : α) → x ∈ xs → β) (z : β) : β :=
   xs.foldlWith' f z 0
 
-theorem foldlWith'_cons' {β : Sort*} {xs : List α} {x : α}
+theorem foldlWith'_cons' {xs : List α} {x : α}
 {f : β → (y : α) → y ∈ (⟨x :: xs⟩ : Array α) → β} {z : β} {i} (h : i ≠ 0) :
 (⟨x :: xs⟩ : Array α).foldlWith' f z i = (⟨xs⟩ : Array α).foldlWith'
 (λ acc x h₁ => f acc x # by simp at h₁; simp [h₁]) z (i - 1) := by
@@ -34,13 +34,13 @@ theorem foldlWith'_cons' {β : Sort*} {xs : List α} {x : α}
     linarith
 
 @[simp]
-theorem foldlWith'_cons {β : Sort*} {xs : List α} {x : α}
+theorem foldlWith'_cons {xs : List α} {x : α}
 {f : β → (y : α) → y ∈ (⟨x :: xs⟩ : Array α) → β} {z : β} {i} :
 (⟨x :: xs⟩ : Array α).foldlWith' f z (i + 1) = (⟨xs⟩ : Array α).foldlWith'
 (λ acc x h₁ => f acc x # by simp at h₁; simp [h₁]) z i :=
   foldlWith'_cons' # by simp
 
-theorem foldlWith_eq_foldlWith_toList {β : Sort*} {f : β → (x : α) → x ∈ xs → β} {z : β} :
+theorem foldlWith_eq_foldlWith_toList {f : β → (x : α) → x ∈ xs → β} {z : β} :
 xs.foldlWith f z = xs.toList.foldlWith (λ acc x h => f acc x # by simp at h; exact h) z := by
   classical
   unfold foldlWith
@@ -73,3 +73,29 @@ xs.foldlWith f z = xs.foldl (λ acc x => if h : x ∈ xs then f acc x h else z) 
 theorem foldlWith_eq_foldl_toList [ha : DecidableEq α] {f : β → (x : α) → x ∈ xs → β} {z : β} :
 xs.foldlWith f z = xs.toList.foldl (λ acc x => if h : x ∈ xs then f acc x h else z) z := by
   simp; exact foldlWith_eq_foldl
+
+def mapWith (xs : Array α) (f : (x : α) → x ∈ xs → β) : Array β :=
+  ⟨xs.toList.mapWith # λ x h => f x # by simp at h; exact h⟩
+
+def inhabited_of_ne_nil (h : xs ≠ #[]) : Inhabited α :=
+  match h₁ : xs with
+  | ⟨[]⟩ => by simp at h
+  | ⟨x :: _⟩ => ⟨x⟩
+
+def inhabited_mapWith_of_ne_nil (f : (x : α) → x ∈ xs → β) (h : xs ≠ #[]) : Inhabited β :=
+  match h₁ : xs with
+  | ⟨[]⟩ => by simp at h
+  | ⟨x :: _⟩ => ⟨f x # by simp⟩
+
+theorem mapWith_eq_mapWith_toList {f : (x : α) → x ∈ xs → β} :
+xs.mapWith f = ⟨xs.toList.mapWith # λ x h => f x # by simp at h; exact h⟩ := rfl
+
+@[simp]
+theorem mapWith_mk {xs : List α} {f : (x : α) → x ∈ Array.mk xs → β} :
+(Array.mk xs).mapWith f = ⟨xs.mapWith (λ x h => f x # by simpa)⟩ := rfl
+
+theorem mapWith_eq_map [ha : DecidableEq α] {f : (x : α) → x ∈ xs → β} :
+xs.mapWith f = if h : xs = #[] then #[] else
+xs.map (λ x => if h₁ : x ∈ xs then f x h₁ else
+inhabited_mapWith_of_ne_nil f h |>.default) := by
+  rcases xs with ⟨xs⟩; simp [xs.mapWith_eq_map]; cases xs <;> simp
