AP/Util/Data/Trie/Raw0.lean
@@ -43,7 +43,7 @@ inductive WF : Raw₀ α β → Prop where
 theorem WF.mp {t : Raw₀ α β} [wf : t.WF] : t.mp.WF := by
   cases wf; assumption
 
-theorem WF.wf_get? {t : Raw₀ α β} [wf : t.WF]
+theorem WF.get? {t : Raw₀ α β} [wf : t.WF]
 {k t'} (h : t.mp.get? k = some t') : t'.WF := by
   cases wf; nm val mp h₁ h₂ h₃; exact h₃ h
 
@@ -121,7 +121,7 @@ def recAux {γ : Raw₀ α β → Sort*} (t : Raw₀ α β) (wf : t.WF)
 mp.WF → (∀ i t, mp.get? i = some t → γ t) → γ (mk val mp)) : γ t :=
   match t with
   | .mk val mp => motive val mp wf.mp #
-    λ i t h => t.recAux (wf.wf_get? h) motive
+    λ i t h => t.recAux (wf.get? h) motive
 termination_by t.depthAux
 decreasing_by exact depthAux_le h
 
@@ -147,13 +147,13 @@ theorem rec'_mk {γ : Raw₀ α β → Sort*} {val mp} [wf : (⟨val, mp⟩ : Ra
 {motive : ∀ (val : Option β) (mp : DHashMap.Raw α (λ _ => Raw₀ α β)),
 mp.WF → (∀ i t, mp.get? i = some t → γ t) → γ (mk val mp)} :
 (⟨val, mp⟩ : Raw₀ α β).rec' motive =
-motive val mp wf.mp (λ _ t h => t.rec' (wf := wf.wf_get? h) motive) := by
+motive val mp wf.mp (λ _ t h => t.rec' (wf := wf.get? h) motive) := by
   simp_rw [rec', recAux]
 
 @[simp]
 theorem depth_mk {val mp} [wf : (⟨val, mp⟩ : Raw₀ α β).WF] :
 (⟨val, mp⟩ : Raw₀ α β).depth = mp.foldWith wf.mp
-(λ acc _ (t' : Raw₀ α β) h => max acc # 1 + t'.depth (wf := wf.wf_get? h)) 0 := by
+(λ acc _ (t' : Raw₀ α β) h => max acc # 1 + t'.depth (wf := wf.get? h)) 0 := by
   unfold depth; simp
 
 @[simp]
@@ -161,13 +161,13 @@ theorem depth_empty : (∅ : Raw₀ α β).depth = 0 := by
   simp [empty_def]
 
 theorem depth_lt [wf : t.WF] {k t'} (h : t.mp.get? k = some t') :
-t'.depth (wf := wf.wf_get? h) < t.depth := by
+t'.depth (wf := wf.get? h) < t.depth := by
   classical
   rcases t with ⟨val, mp⟩
   simp at h ⊢
   have h₁ := DHashMap.Raw.mem_toList_iff_get?_eq_some wf.mp |>.mpr h
   dsimp at h₁
-  have h₂ := wf.wf_get? h
+  have h₂ := wf.get? h
   rw [DHashMap.Raw.foldWith_eq_foldlWith_toList, List.foldlWith_max_eq_max?_mapWith]
   apply Nat.lt_of_succ_le
   change (⟨k, t'⟩ : Σ _, _).snd.depth + 1 ≤ _
@@ -175,3 +175,6 @@ t'.depth (wf := wf.wf_get? h) < t.depth := by
   simp
   use k, t', h₁
   rw [add_comm]
+
+theorem WF.of_mem_toList [wf : t.WF] {p} (h : p ∈ t.mp.toList) : p.2.WF := by
+  rw [DHashMap.Raw.mem_toList_iff_get?_eq_some wf.mp] at h; exact wf.get? h
